compiler/inference/unify_cvScript.sml
@@ -9,9 +9,42 @@ val _ = new_theory "unify_cv";
 
 val tcvwalk_pre_def = cv_trans_pre tcvwalk_thm;
 
+Theorem tcvwalk_pre:
+  ∀s t. cwfs s ⇒ tcvwalk_pre s t
+Proof
+  rpt strip_tac >> drule_then assume_tac $ SRULE[FORALL_PROD]WF_cvwalkR >>
+  ‘∀p. FST p = s ⇒ (λ(s0,n). tcvwalk_pre s0 n) p’
+    suffices_by simp[FORALL_PROD] >>
+  IMP_RES_THEN ho_match_mp_tac relationTheory.WF_INDUCTION_THM >>
+  simp[FORALL_PROD] >> qx_gen_tac ‘n’ >>
+  strip_tac >>
+  simp[Once tcvwalk_pre_def] >> rw[] >>
+  drule (SRULE[FORALL_PROD]cvwalk_ensures_decrease) >>
+  simp[cvwalk_code_def, AllCaseEqs()]
+QED
+
 val tcwalk_pre_def = cv_trans_pre tcwalk_def;
 
+Theorem tcwalk_pre:
+  cwfs s ⇒ tcwalk_pre s t
+Proof
+  simp[tcwalk_pre_def, tcvwalk_pre]
+QED
+
 val tcocwl_pre_def = cv_trans_pre tcocwl_thm;
+
+Theorem tcocwl_pre:
+  ∀s n wl. cwfs s ⇒ tcocwl_pre s n wl
+Proof
+  rpt strip_tac >> drule_then assume_tac WF_kcocwlR >>
+  ‘∀t. FST t = s ⇒ (λ(s,n,wl). tcocwl_pre s n wl) t’
+    suffices_by simp[FORALL_PROD] >>
+  IMP_RES_THEN ho_match_mp_tac relationTheory.WF_INDUCTION_THM >>
+  simp[FORALL_PROD] >> qx_genl_tac [‘n’, ‘wl’] >> strip_tac >>
+  simp[Once tcocwl_pre_def] >> rw[] >> simp[tcwalk_pre] >>
+  drule (SRULE[FORALL_PROD]kcocwl_ensures_decrease) >>
+  simp[kcocwl_code_def]
+QED
 
 val tcunify_pre_def = cv_trans_pre tcunify_thm;
 
@@ -23,6 +56,8 @@ Proof
   qsuff_tac ‘cwfs s ⇒ cunify_pre s t1 t2’
   >- metis_tac [cunify_pre_def]
   \\ gvs [cunify_pre_def]
+  \\ simp[Once tcunify_pre_def]
+  \\ rpt strip_tac
   \\ cheat
 QED
 
